Meta: move definitions to subfolder

Engine/Meta/Meta.v
@@ -12,11 +12,10 @@ Require Import List.
 Import ListNotations.
 
 From Linden Require Import Regex Chars Semantics Tree.
-From Linden Require Import FunctionalUtils FunctionalSemantics.
+From Linden Require Import FunctionalUtils.
 From Linden Require Import Parameters LWParameters.
 From Linden Require Import StrictSuffix Prefix.
-From Linden Require Import PikeSubset SeenSets.
-From Linden Require Import Correctness FunctionalPikeVM.
+From Linden Require Import EngineSpec.
 From Warblre Require Import Base RegExpRecord.
 
 
@@ -24,50 +23,9 @@ Section Meta.
   Context {params: LindenParameters}.
   Context (rer: RegExpRecord).
 
-(* We define what it means to be a regex engine and show that our engines follow these definitions. *)
-Section Engines.
-  Context {VMS: VMSeen}.
-  Context {strs: StrSearch}.
-
-(* interface of an anchored, executable engine *)
-Class AnchoredEngine := {
-  exec: regex -> input -> option leaf;
-
-  (* asserts the supported subset of regexes *)
-  supported_regex: regex -> Prop;
-
-  (* the execution follows the backtracking tree semantics *)
-  exec_correct: forall r inp tree ol,
-    supported_regex r ->
-    is_tree rer [Areg r] inp Groups.GroupMap.empty forward tree ->
-    (first_leaf tree inp = ol <-> exec r inp = ol)
-}.
-
-(* we show that the PikeVM fits the scheme of an anchored engine *)
-#[refine]
-Instance PikeVMAnchoredEngine: AnchoredEngine := {
-  exec r inp := match pike_vm_match rer r inp with
-                | OutOfFuel => None
-                | Finished res => res
-                end;
-  supported_regex := pike_regex;
-}.
-  (* exec_correct *)
-  intros r inp tree ol Hsubset Htree.
-  pose proof (pike_vm_match_terminates rer r inp Hsubset) as [res Hmatch].
-  rewrite Hmatch.
-  split.
-  - intros Hleaf.
-    subst. eauto using pike_vm_match_correct, pike_vm_correct.
-  - intros <-.
-    symmetry. eauto using pike_vm_match_correct, pike_vm_correct.
-Qed.
-End Engines.
-
-Existing Instance literal_EqDec.
 (* for each input position we run the anchored engine and return the earliest match *)
-Fixpoint search_from {engine:AnchoredEngine} (r: regex) (next: string) (prev: string): option leaf :=
-  match (exec r (Input next prev)) with
+Fixpoint search_from {engine:AnchoredEngine rer} (r: regex) (next: string) (prev: string): option leaf :=
+  match (exec rer r (Input next prev)) with
   | Some leaf => Some leaf
   | None => match next with
             | [] => None
@@ -81,11 +39,12 @@ Definition pref_str (i: input) : string :=
   end.
 
 (* the string-quadratic algorithm described in RegExpBuiltinExec *)
-Definition BuiltinExec {engine:AnchoredEngine} (r:regex) (inp:input) : option leaf :=
+Definition BuiltinExec {engine:AnchoredEngine rer} (r:regex) (inp:input) : option leaf :=
   search_from r (next_str inp) (pref_str inp).
 
+
 (* prefixed version *)
-Definition BuiltinExecPrefixed {strs:StrSearch} {engine:AnchoredEngine} (r:regex) (inp:input) : option leaf :=
+Definition BuiltinExecPrefixed {strs:StrSearch} {engine:AnchoredEngine rer} (r:regex) (inp:input) : option leaf :=
   let lit := extract_literal rer r in
   if lit == Impossible then None else
     let p := prefix lit in
@@ -95,9 +54,24 @@ Definition BuiltinExecPrefixed {strs:StrSearch} {engine:AnchoredEngine} (r:regex
     | Some i => search_from r (next_str i) (pref_str i)
     end.
 
-Lemma search_from_before_jump_eq {strs:StrSearch} {engine:AnchoredEngine}:
+
+(* Fixpoint jump_try {strs:StrSearch} {engine:AnchoredEngine} (r:regex) (p:string) (next pref:string) : option leaf :=
+  (* we skip the initial input that does not match the prefix *)
+  match (input_search p (Input next pref)) with
+  | None => None (* if prefix is not present anywhere, then we cannot match *)
+  | Some (Input  =>
+      match (exec r (Input next pref)) with
+      | Some leaf => Some leaf
+      | None => match next with
+                | [] => None
+                | c::t => jump_try r p t (c::pref)
+                end
+      end
+  end. *)
+
+Lemma search_from_before_jump_eq {strs:StrSearch} {engine:AnchoredEngine rer}:
   forall i r inp inp',
-    supported_regex r ->
+    supported_regex rer r ->
     input_search (prefix (extract_literal rer r)) inp = Some inp' ->
     input_prefix i inp' forward ->
     input_prefix inp i forward ->
@@ -111,7 +85,7 @@ Proof.
     specialize (IHHprefix Hsearch).
     unfold advance_input in H. destruct inp1 as [next1 pref1] eqn:Hinp1, next1 eqn:Hnext1; [easy|].
     inversion H. rewrite <-H1 in IHHprefix.
-    assert (Hnone: exec r (Input (t :: s) pref1) = None). {
+    assert (Hnone: exec rer r (Input (t :: s) pref1) = None). {
       assert (Hbetween: input_between inp inp3 inp1). {
         rewrite input_prefix_strict_suffix in Hprefix, Hlow.
         split; destruct Hprefix, Hlow; subst; eauto using ss_next', ss_advance.
@@ -126,12 +100,12 @@ Proof.
     eauto using ip_prev'.
 Qed.
 
-Lemma input_search_exec_none {strs:StrSearch} {engine:AnchoredEngine}:
+Lemma input_search_exec_none {strs:StrSearch} {engine:AnchoredEngine rer}:
   forall i r inp,
-    supported_regex r ->
+    supported_regex rer r ->
     input_search (prefix (extract_literal rer r)) inp = None ->
     input_prefix inp i forward ->
-    exec r i = None.
+    exec rer r i = None.
 Proof.
   intros i r inp Hsubset Hsearch Hlow.
   rewrite input_prefix_strict_suffix in Hlow.
@@ -140,9 +114,9 @@ Proof.
   eauto using input_search_not_found, extract_literal_prefix_contra.
 Qed.
 
-Lemma search_from_none_prefix {strs:StrSearch} {engine:AnchoredEngine}:
+Lemma search_from_none_prefix {strs:StrSearch} {engine:AnchoredEngine rer}:
   forall i r inp,
-    supported_regex r ->
+    supported_regex rer r ->
     input_search (prefix (extract_literal rer r)) inp = None ->
     input_prefix inp i forward ->
     search_from r (next_str i) (pref_str i) = None.
@@ -156,11 +130,11 @@ Proof.
     all: eauto using ip_prev'.
 Qed.
 
-Lemma input_search_exec_impossible {strs:StrSearch} {engine:AnchoredEngine}:
+Lemma input_search_exec_impossible {strs:StrSearch} {engine:AnchoredEngine rer}:
   forall inp r,
-    supported_regex r ->
+    supported_regex rer r ->
     extract_literal rer r = Impossible ->
-    exec r inp = None.
+    exec rer r inp = None.
 Proof.
   intros inp r Hsubset Hextract.
   pose proof (is_tree_productivity rer [Areg r] inp Groups.GroupMap.empty forward) as [tree Htree].
@@ -168,9 +142,9 @@ Proof.
   eauto using extract_literal_impossible.
 Qed.
 
-Lemma search_from_impossible_prefix {strs:StrSearch} {engine:AnchoredEngine}:
+Lemma search_from_impossible_prefix {strs:StrSearch} {engine:AnchoredEngine rer}:
   forall inp r,
-    supported_regex r ->
+    supported_regex rer r ->
     extract_literal rer r = Impossible ->
     search_from r (next_str inp) (pref_str inp) = None.
 Proof.
@@ -179,9 +153,9 @@ Proof.
   induction next; intros pref; simpl; erewrite input_search_exec_impossible; eauto.
 Qed.
 
-Theorem builtin_exec_equiv {strs:StrSearch} {engine:AnchoredEngine}:
+Theorem builtin_exec_equiv {strs:StrSearch} {engine:AnchoredEngine rer}:
   forall r inp,
-    supported_regex r ->
+    supported_regex rer r ->
     BuiltinExec r inp = BuiltinExecPrefixed r inp.
 Proof.
   intros r inp Hsubset.
