Engine/Meta/EngineSpec.v
@@ -1,0 +1,54 @@
+(** * Engine specification *)
+
+(* This module describes what it means to be a regex engine. *)
+(* We also show that our engines follow these definitions. *)
+
+Require Import List.
+Import ListNotations.
+
+From Linden Require Import Regex Chars Semantics Tree.
+From Linden Require Import Parameters LWParameters.
+From Linden Require Import PikeSubset SeenSets FunctionalPikeVM.
+From Linden Require Import Correctness.
+From Warblre Require Import Base RegExpRecord.
+
+
+Section Engines.
+  Context {VMS: VMSeen}.
+  Context {params: LindenParameters}.
+  Context (rer: RegExpRecord).
+
+(* interface of an anchored, executable engine *)
+Class AnchoredEngine := {
+  exec: regex -> input -> option leaf;
+
+  (* asserts the supported subset of regexes *)
+  supported_regex: regex -> Prop;
+
+  (* the execution follows the backtracking tree semantics *)
+  exec_correct: forall r inp tree ol,
+    supported_regex r ->
+    is_tree rer [Areg r] inp Groups.GroupMap.empty forward tree ->
+    (first_leaf tree inp = ol <-> exec r inp = ol)
+}.
+
+(* we show that the PikeVM fits the scheme of an anchored engine *)
+#[refine]
+Instance PikeVMAnchoredEngine: AnchoredEngine := {
+  exec r inp := match pike_vm_match rer r inp with
+                | OutOfFuel => None
+                | Finished res => res
+                end;
+  supported_regex := pike_regex;
+}.
+  (* exec_correct *)
+  intros r inp tree ol Hsubset Htree.
+  pose proof (pike_vm_match_terminates rer r inp Hsubset) as [res Hmatch].
+  rewrite Hmatch.
+  split.
+  - intros Hleaf.
+    subst. eauto using pike_vm_match_correct, pike_vm_correct.
+  - intros <-.
+    symmetry. eauto using pike_vm_match_correct, pike_vm_correct.
+Qed.
+End Engines.
